cogent/examples/wa_connect/WordArray_UpdCCorres.thy
@@ -6,6 +6,63 @@ theory WordArray_UpdCCorres
 begin
 
 context WordArray begin
+(*
+abbreviation "w_val h w \<equiv> values_C (h w)"
+abbreviation "w_len h w \<equiv> SCAST(32 signed \<rightarrow> 32) (len_C (h w))"
+
+abbreviation "w_p s w \<equiv> w_val (heap_WordArray_u32_C s) w"
+abbreviation "w_l s w \<equiv> w_len (heap_WordArray_u32_C s) w"
+
+section "Helper Lemma for Word Array Existence and Validity"
+ 
+definition valid_c_wordarray
+  where
+  "valid_c_wordarray s w \<equiv> is_valid_WordArray_u32_C s w \<and> 
+                            (\<forall>i < w_l s w. is_valid_w32 s ((w_p s w) +\<^sub>p uint i)) "
+
+definition valid_cogent_wordarray
+  where
+  "valid_cogent_wordarray \<sigma> s w \<equiv> (\<exists>len arr. len = w_l s w \<and> arr = ptr_val (w_p s w) \<and> 
+                                    \<sigma> (ptr_val w) = option.Some (UAbstract (WAU32 len arr)) \<and> 
+                                   (\<forall>i < len. \<sigma> (arr + 4 * i) = option.Some (UPrim (LU32 (heap_w32 s ((w_p s w) +\<^sub>p uint i))))))"
+
+definition valid_wordarray
+  where
+  "valid_wordarray \<sigma> s w \<equiv> valid_c_wordarray s w \<and> valid_cogent_wordarray \<sigma> s w"
+
+
+lemma well_typed_related_wordarray: "\<And>\<sigma> st x x' a ts s r w.
+       \<lbrakk>(\<sigma>, st) \<in> state_rel; val_rel x (x':: WordArray_u32_C ptr); abs_typing_u a ts\<rbrakk>
+       \<Longrightarrow> valid_wordarray \<sigma> st x'"
+  apply (unfold valid_wordarray_def valid_c_wordarray_def valid_cogent_wordarray_def)
+  apply (clarsimp simp: val_rel_simp)
+  apply (erule u_t_recE)
+  apply (erule u_t_r_consE; clarsimp simp: \<Xi>_def wordarray_put2_0_type_def abbreviatedType1_def)
+  apply (erule u_t_p_absE; clarsimp)
+  apply (clarsimp simp: abs_typing'_def)
+  apply (case_tac a; clarsimp)
+  apply (clarsimp simp: state_rel_def heap_rel_def heap_rel_ptr_meta heap_rel_ptr_w32_meta)
+  apply (drule_tac p = "arr_C x'" and uv = "UAbstract (WAU32 x11 x12)" in all_heap_rel_ptrD; 
+         clarsimp simp: type_rel_simp abs_repr'_def val_rel_simp is_valid_simp heap_simp)
+  apply (rule conjI)
+   apply clarsimp
+   apply (erule_tac x = i in allE)
+   apply (erule_tac x = i in allE)
+   apply clarsimp
+   apply (drule_tac uv = "UPrim (LU32 x)" and 
+                     p = "values_C (heap_WordArray_u32_C st (arr_C x')) +\<^sub>p uint i"
+                     in all_heap_rel_ptrD;
+          clarsimp simp: ptr_add_def mult.commute type_rel_simp)
+  apply clarsimp
+  apply (erule_tac x = i in allE)
+  apply (erule_tac x = i in allE)
+  apply clarsimp
+  apply (drule_tac uv = "UPrim (LU32 x)" and 
+                    p = "values_C (heap_WordArray_u32_C st (arr_C x')) +\<^sub>p uint i"
+                    in all_heap_rel_ptrD;
+         clarsimp simp: ptr_add_def mult.commute type_rel_simp val_rel_simp)
+  done
+*)
 section "Correspondence Lemmas Between Update Semantics and C"
 
 lemma upd_C_wordarray_put2_corres:
@@ -17,10 +74,10 @@ lemma upd_C_wordarray_put2_corres:
           od)
          \<xi>0 \<gamma> \<Xi> \<Gamma>' \<sigma> st"
   apply (rule afun_corres; simp)
-  apply (clarsimp simp: abs_rel_def; rename_tac r w)
   apply (thin_tac "i < length \<gamma>")
   apply (thin_tac "val_rel (\<gamma> ! i) v'")
-  apply (thin_tac "\<Gamma>' ! i = option.Some (prod.fst (prod.snd (\<Xi> ''wordarray_put2_0'')))")
+  apply (thin_tac "\<Gamma>' ! i = _")
+  apply (clarsimp simp: abs_rel_def; rename_tac r w)
   apply (clarsimp simp: val_rel_simp \<Xi>_def wordarray_put2_0_type_def abbreviatedType5_def)
   apply (erule upd.u_t_recE)
   apply (erule upd.u_t_r_consE; clarsimp)+
@@ -83,7 +140,7 @@ lemma upd_C_wordarray_length_corres:
   apply (clarsimp simp: abs_rel_def; rename_tac r w)
   apply (thin_tac "i < length \<gamma>")
   apply (thin_tac "val_rel (\<gamma> ! i) v'")
-  apply (thin_tac "\<Gamma>' ! i = option.Some (prod.fst (prod.snd (\<Xi> ''wordarray_length_0'')))")
+  apply (thin_tac "\<Gamma>' ! i = _")
   apply (clarsimp simp: val_rel_simp \<Xi>_def wordarray_length_0_type_def)
   apply (erule upd.u_t_p_absE; clarsimp simp: abs_typing_u_def)
   apply (case_tac a; clarsimp)
@@ -116,7 +173,7 @@ lemma upd_C_wordarray_get_corres:
   apply (clarsimp simp: abs_rel_def; rename_tac r w)
   apply (thin_tac "i < length \<gamma>")
   apply (thin_tac "val_rel (\<gamma> ! i) v'")
-  apply (thin_tac "\<Gamma>' ! i = option.Some (prod.fst (prod.snd (\<Xi> ''wordarray_get_0'')))")
+  apply (thin_tac "\<Gamma>' ! i = _")
   apply (clarsimp simp: val_rel_simp \<Xi>_def wordarray_get_0_type_def abbreviatedType6_def)
   apply (erule upd.u_t_recE)
   apply (erule upd.u_t_r_consE; clarsimp)+
@@ -149,6 +206,23 @@ lemma upd_C_wordarray_get_corres:
   apply blast
   done
 
+lemma
+" \<And>v' i \<gamma> \<Gamma>' \<sigma> s.
+    \<lbrakk>i < length \<gamma>; val_rel (\<gamma> ! i) v';
+     \<Gamma>' ! i = option.Some (prod.fst (prod.snd (\<Xi> ''wordarray_map_no_break_0'')))\<rbrakk>
+    \<Longrightarrow> update_sem_init.corres abs_typing_u abs_repr_u (Generated.state_rel abs_repr_u)
+         (App (AFun ''wordarray_map_no_break_0'' []) (Var i)) (do x <- main_pp_inferred.wordarray_map_no_break_0' v';
+gets (\<lambda>s. x)
+                                                                od)
+         \<xi>1 \<gamma> \<Xi>  \<Gamma>' \<sigma> s"
+  apply (rule afun_corres; clarsimp)
+  apply (clarsimp simp: abs_rel_def)
+  apply (thin_tac "i < length \<gamma>")
+  apply (thin_tac "val_rel (\<gamma> ! i) v'")
+  apply (thin_tac "\<Gamma>' ! i = _")
+  apply clarsimp
+  apply (clarsimp simp: val_rel_simp)
+  oops
 
 
 lemma
@@ -159,15 +233,509 @@ lemma
          (App (AFun ''wordarray_fold_no_break_0'' []) (Var i)) (do x <- main_pp_inferred.wordarray_fold_no_break_0' v';
 gets (\<lambda>s. x)
                                                                 od)
-         \<xi>0 \<gamma> \<Xi>  \<Gamma>' \<sigma> s"
-  apply (rule afun_corres; simp)
+         \<xi>1 \<gamma> \<Xi>  \<Gamma>' \<sigma> s"
+  apply (rule afun_corres; clarsimp)
   apply (clarsimp simp: abs_rel_def')
   apply (thin_tac "i < length \<gamma>")
   apply (thin_tac "val_rel (\<gamma> ! i) v'")
-  apply (thin_tac "\<Gamma>' ! i = option.Some (prod.fst (prod.snd (\<Xi> ''wordarray_fold_no_break_0'')))")
+  apply (thin_tac "\<Gamma>' ! i = _")
   apply clarsimp
   apply (clarsimp simp: val_rel_simp)
-(*
+  apply (erule upd.u_t_recE)
+  apply (clarsimp simp: \<Xi>_def wordarray_fold_no_break_0_type_def abbreviatedType1_def)
+  apply (erule upd.u_t_r_consE; clarsimp)+
+  apply (erule upd.u_t_primE; subst (asm) lit_type.simps; clarsimp)+
+  apply (erule upd.u_t_r_emptyE)
+  apply (erule upd.u_t_unitE)
+  apply (case_tac "sint (t5_C.f_C x') \<noteq> sint FUN_ENUM_mul \<and> sint (t5_C.f_C x') \<noteq> sint FUN_ENUM_sum")
+   apply (clarsimp simp: cogent_function_val_rel
+                         FUN_ENUM_sum_def
+                         FUN_ENUM_dec_def
+                         FUN_ENUM_inc_def
+                         FUN_ENUM_mul_def
+                         FUN_ENUM_dec_arr_def
+                         FUN_ENUM_inc_arr_def
+                         FUN_ENUM_mul_arr_def
+                         FUN_ENUM_sum_arr_def
+                         FUN_ENUM_wordarray_get_0_def
+                         FUN_ENUM_wordarray_length_0_def
+                         FUN_ENUM_wordarray_put2_0_def
+                         FUN_ENUM_wordarray_fold_no_break_0_def
+                         FUN_ENUM_wordarray_map_no_break_0_def
+                         FUN_ENUM_wordarray_get_u32_def
+                         FUN_ENUM_wordarray_length_u32_def
+                         FUN_ENUM_wordarray_put2_u32_def)
+   apply (rule FalseE) 
+   apply (thin_tac "_ \<in> state_rel")
+   apply (thin_tac "sint (t5_C.f_C x') \<noteq> 4")
+   apply (thin_tac "sint (t5_C.f_C x') \<noteq> 6")
+   apply (thin_tac "upd.uval_typing _ _ (UPtr _ _) _ _ _")
+   apply (thin_tac "_ = _")+
+   apply clarsimp
+   apply (erule disjE)
+    apply clarsimp
+    apply (erule upd.u_t_funE')
+    apply (clarsimp simp: dec_def)
+    apply (clarsimp simp: subtyping_simps(4) 
+                          subtyping.simps[of _ _ "TPrim (Num U32)", simplified]
+                          subtyping.simps[of _ "TRecord _ _ ", simplified]
+                          subtyping.simps[of _ "TPrim (Num U32)", simplified]
+                          subtyping.simps[of _ "TUnit", simplified]
+                          kinding_simps(5, 9))
+    apply (erule typing_takeE)+
+    apply (erule typing_letE)+
+    apply (erule typing_structE)
+    apply clarsimp
+   apply (erule disjE)
+    apply clarsimp
+    apply (erule upd.u_t_funE')
+    apply (clarsimp simp: inc_def)
+    apply (clarsimp simp: subtyping_simps(4) 
+                          subtyping.simps[of _ _ "TPrim (Num U32)", simplified]
+                          subtyping.simps[of _ "TRecord _ _ ", simplified]
+                          subtyping.simps[of _ "TPrim (Num U32)", simplified]
+                          subtyping.simps[of _ "TUnit", simplified]
+                          kinding_simps(5, 9))
+    apply (erule typing_takeE)+
+    apply (erule typing_letE)+
+    apply (erule typing_structE)
+    apply clarsimp
+   apply (erule disjE)
+    apply clarsimp
+    apply (erule upd.u_t_funE')     
+    apply (clarsimp simp: dec_arr_def)
+    apply (clarsimp simp: subtyping_simps(4) 
+                          subtyping.simps[of _ _ "TPrim (Num U32)", simplified]
+                          subtyping.simps[of _ "TRecord _ _ ", simplified]
+                          subtyping.simps[of _ "TPrim (Num U32)", simplified]
+                          subtyping.simps[of _ "TUnit", simplified]
+                          kinding_simps(5, 9))     
+    apply (erule typing_letE)
+    apply (erule typing_letbE)
+    apply (erule typing_letE)+
+    apply (erule typing_appE)+
+    apply (erule typing_afunE)+
+    apply (thin_tac "_, _, _ \<turnstile> _ : _")+
+    apply (clarsimp simp: wordarray_map_no_break_0_type_def abbreviatedType2_def)
+   apply (erule disjE)
+    apply clarsimp
+    apply (erule upd.u_t_funE')
+    apply (clarsimp simp: inc_arr_def)
+    apply (clarsimp simp: subtyping_simps(4) 
+                          subtyping.simps[of _ _ "TPrim (Num U32)", simplified]
+                          subtyping.simps[of _ "TRecord _ _ ", simplified]
+                          subtyping.simps[of _ "TPrim (Num U32)", simplified]
+                          subtyping.simps[of _ "TUnit", simplified]
+                          kinding_simps(5, 9)) 
+    apply (erule typing_letE)
+    apply (erule typing_letbE)
+    apply (erule typing_letE)+
+    apply (erule typing_appE)+
+    apply (erule typing_afunE)+
+    apply (thin_tac "_, _, _ \<turnstile> _ : _")+
+    apply (clarsimp simp: wordarray_map_no_break_0_type_def abbreviatedType2_def)
+   apply (erule disjE)
+    prefer 2
+    apply (erule disjE)
+     prefer 2
+     apply (erule disjE)
+      apply clarsimp
+      apply (erule upd.u_t_afunE; clarsimp)
+      apply (clarsimp simp: subtyping_simps(4) 
+                            subtyping.simps[of _ _ "TPrim (Num U32)", simplified]
+                            wordarray_get_0_type_def abbreviatedType6_def
+                            subtyping_simps(6))
+     apply (erule disjE)
+      apply clarsimp
+      apply (erule upd.u_t_afunE; clarsimp)
+      apply (clarsimp simp: subtyping_simps(4) 
+                            subtyping.simps[of _ _ "TPrim (Num U32)", simplified]
+                            wordarray_put2_0_type_def)
+     apply (erule disjE)
+      apply clarsimp
+      apply (erule upd.u_t_funE'; clarsimp)
+      apply (clarsimp simp: subtyping_simps(4)
+                            subtyping.simps[of _ "TRecord _ _ ", simplified]
+                            subtyping.simps[of _ _ "TPrim (Num U32)", simplified]
+                            subtyping.simps[of _ "TPrim (Num U32)", simplified]
+                            subtyping.simps[of _ "TUnit", simplified]
+                            kinding_simps(5, 9))
+      apply (clarsimp simp: wordarray_get_u32_def)
+      apply (erule typing_letE)
+      apply (erule typing_appE)
+      apply (erule typing_afunE)
+      apply (clarsimp simp: wordarray_get_0_type_def abbreviatedType6_def)
+      apply (erule typing_varE)+
+      apply (clarsimp simp: split_conv_all_nth weakening_conv_all_nth empty_def)
+      apply (erule_tac x = 0 in allE)+
+      apply (clarsimp simp: weakening_comp.simps split_comp.simps)
+      apply (erule disjE; clarsimp)
+     apply (erule disjE)
+      apply clarsimp
+      apply (erule upd.u_t_afunE; clarsimp)
+      apply (clarsimp simp: subtyping_simps(4) 
+                            subtyping.simps[of _ _ "TPrim (Num U32)", simplified]
+                            subtyping.simps[of _ "TRecord _ _ ", simplified]
+                            wordarray_length_0_type_def)
+     apply (erule disjE)
+      apply clarsimp
+      apply (erule upd.u_t_funE'; clarsimp)
+      apply (clarsimp simp: subtyping_simps(4)
+                            subtyping.simps[of _ "TRecord _ _ ", simplified]
+                            subtyping.simps[of _ _ "TPrim (Num U32)", simplified]
+                            subtyping.simps[of _ "TPrim (Num U32)", simplified]
+                            subtyping.simps[of _ "TUnit", simplified]
+                            kinding_simps(5, 9))
+      apply (clarsimp simp: wordarray_put2_u32_def)
+      apply (erule typing_letE)
+      apply (erule typing_appE)
+      apply (erule typing_afunE)
+      apply (clarsimp simp: wordarray_put2_0_type_def abbreviatedType5_def)
+     apply (erule disjE)
+      apply clarsimp
+      apply (erule upd.u_t_funE'; clarsimp)
+      apply (clarsimp simp: subtyping_simps(4)
+                            subtyping.simps[of _ "TRecord _ _ ", simplified]
+                            subtyping.simps[of _ _ "TPrim (Num U32)", simplified]
+                            subtyping.simps[of _ "TPrim (Num U32)", simplified]
+                            subtyping.simps[of _ "TUnit", simplified]
+                            kinding_simps(5, 9))
+      apply (clarsimp simp: wordarray_length_u32_def)
+      apply (erule typing_letE)
+      apply (erule typing_appE)
+      apply (erule typing_afunE)
+      apply (clarsimp simp: wordarray_length_0_type_def)
+      apply (erule typing_varE)+
+      apply (clarsimp simp: split_conv_all_nth weakening_conv_all_nth empty_def)
+      apply (erule_tac x = 0 in allE)+
+      apply (clarsimp simp: weakening_comp.simps split_comp.simps)
+      apply (erule disjE; clarsimp)
+     apply (erule disjE)
+      apply clarsimp
+      apply (erule upd.u_t_afunE; clarsimp)
+      apply (clarsimp simp: subtyping_simps(4) 
+                            subtyping.simps[of _ _ "TPrim (Num U32)", simplified]
+                            subtyping.simps[of _ "TRecord _ _ ", simplified]
+                            wordarray_map_no_break_0_type_def)
+     apply clarsimp
+     apply (erule upd.u_t_afunE; clarsimp)
+     apply (clarsimp simp: subtyping_simps(4) 
+                           subtyping.simps[of _ _ "TPrim (Num U32)", simplified]
+                           subtyping.simps[of _ "TRecord _ _ ", simplified])
+    apply clarsimp
+    apply (erule upd.u_t_funE')
+    apply (clarsimp simp: subtyping_simps(4) 
+                          subtyping.simps[of _ _ "TPrim (Num U32)", simplified]
+                          subtyping.simps[of _ "TRecord _ _ ", simplified]
+                          subtyping.simps[of _ "TPrim (Num U32)", simplified]
+                          subtyping.simps[of _ "TUnit", simplified]
+                          kinding_simps(5, 9))
+    apply (thin_tac "_ \<or> _")+
+    apply (clarsimp simp: sum_arr_def)
+    apply (erule typing_letE)
+    apply (erule typing_letE)
+    apply (erule typing_varE)
+    apply (thin_tac "_, _, (_ #_) \<turnstile> _ : _")
+    apply (erule typing_appE)
+    apply (erule typing_afunE)
+    apply (erule typing_varE)
+    apply (clarsimp simp: split_conv_all_nth weakening_conv_all_nth empty_def wordarray_length_0_type_def)
+    apply (erule_tac x= 0 in allE)+
+    apply clarsimp
+    apply (clarsimp simp: weakening_comp.simps split_comp.simps neq_Nil_lengthI)
+    apply (erule disjE; clarsimp)+
+   apply clarsimp
+   apply (erule upd.u_t_funE')
+   apply (clarsimp simp: subtyping_simps(4) 
+                         subtyping.simps[of _ _ "TPrim (Num U32)", simplified]
+                         subtyping.simps[of _ "TRecord _ _ ", simplified]
+                         subtyping.simps[of _ "TPrim (Num U32)", simplified]
+                         subtyping.simps[of _ "TUnit", simplified]
+                         kinding_simps(5, 9))
+   apply (thin_tac "_ \<or> _")+
+   apply (clarsimp simp: mul_arr_def)
+   apply (erule typing_letE)
+   apply (erule typing_letE)
+   apply (erule typing_varE)
+   apply (thin_tac "_, _, (_ #_) \<turnstile> _ : _")
+   apply (erule typing_appE)
+   apply (erule typing_afunE)
+   apply (erule typing_varE)
+   apply (clarsimp simp: split_conv_all_nth weakening_conv_all_nth empty_def wordarray_length_0_type_def)
+   apply (erule_tac x= 0 in allE)+
+   apply clarsimp
+   apply (clarsimp simp: weakening_comp.simps split_comp.simps neq_Nil_lengthI)
+   apply (erule disjE; clarsimp)+
+  apply clarsimp
+  apply (erule upd.u_t_p_absE; clarsimp)
+  apply (clarsimp simp: wordarray_fold_no_break_0'_def)
+  apply (subst unknown_bind_ignore)+
+  apply clarsimp
+  apply wp 
+      apply (clarsimp simp: split_def unknown_bind_ignore)
+      apply (subst whileLoop_add_inv
+              [where M = "\<lambda>((_, r), _). unat (t5_C.to_C x') - unat r" and 
+                     I = "\<lambda>(a, b) s. 
+                        (\<exists>f ts. cogent_function_val_rel x (sint (t5_C.f_C x')) \<and> x = UFunction f ts \<and>
+                        upd_wa_foldnb_bod_0 \<sigma> (ptr_val (t5_C.arr_C x')) (t5_C.frm_C x') b (Fun f ts)
+                          (UPrim (LU32 (t5_C.acc_C x')), RPrim (Num U32)) (UUnit, RUnit)
+                          (\<sigma>, UPrim (LU32 (t3_C.acc_C a)))) \<and> (\<sigma>, s) \<in> state_rel \<and> t5_C.frm_C x' \<le> b \<and>
+                        ret = min (t5_C.to_C x') ((SCAST(32 signed \<rightarrow> 32))(len_C (heap_WordArray_u32_C s (t5_C.arr_C x')))) \<and>
+                        (t5_C.frm_C x' \<le> ret \<longrightarrow> b \<le> ret) \<and> (t5_C.frm_C x' \<ge> ret \<longrightarrow> b = t5_C.frm_C x')"])
+      apply clarsimp
+      apply (wp; clarsimp simp: split_def unknown_bind_ignore)
+           apply (clarsimp simp: split_def dispatch_t4'_def unknown_bind_ignore)
+           apply wp
+            apply (clarsimp simp: mul'_def unknown_bind_ignore)
+            apply wp
+           apply (clarsimp simp: sum'_def unknown_bind_ignore)
+           apply wp
+          apply wp
+         apply wp
+        apply wp
+       apply (clarsimp simp: split_def cogent_function_val_rel
+                             FUN_ENUM_sum_def
+                             FUN_ENUM_dec_def
+                             FUN_ENUM_inc_def
+                             FUN_ENUM_mul_def
+                             FUN_ENUM_dec_arr_def
+                             FUN_ENUM_inc_arr_def
+                             FUN_ENUM_mul_arr_def
+                             FUN_ENUM_sum_arr_def
+                             FUN_ENUM_wordarray_get_0_def
+                             FUN_ENUM_wordarray_length_0_def
+                             FUN_ENUM_wordarray_put2_0_def
+                             FUN_ENUM_wordarray_fold_no_break_0_def
+                             FUN_ENUM_wordarray_map_no_break_0_def
+                             FUN_ENUM_wordarray_get_u32_def
+                             FUN_ENUM_wordarray_length_u32_def
+                             FUN_ENUM_wordarray_put2_u32_def)
+       apply (thin_tac "upd.uval_typing _ _ _ _ _ _")
+       apply (clarsimp simp: abs_typing_u_def)
+       apply (case_tac a; clarsimp)
+       apply (erule_tac x = b in allE)
+       apply (thin_tac "_ \<in> state_rel")
+       apply (clarsimp simp: state_rel_def heap_rel_def heap_rel_ptr_meta heap_rel_ptr_w32_meta)
+       apply (drule_tac p = "t5_C.arr_C x'" and uv = "UAbstract (WAU32 x11 x12)" in all_heap_rel_ptrD; 
+              clarsimp simp: type_rel_simps is_valid_simp heap_simp abs_repr_u_def val_rel_simps) 
+       apply (drule_tac p = "values_C (heap_WordArray_u32_C s (t5_C.arr_C x')) +\<^sub>p uint b" and 
+                       uv = "UPrim (LU32 x)" in all_heap_rel_ptrD; clarsimp simp: type_rel_simps)
+       apply (rule conjI; clarsimp)
+        apply (rule conjI)
+         apply (rule_tac r = "UPrim (LU32 (t3_C.acc_C aa))" and 
+                       len = "(SCAST(32 signed \<rightarrow> 32) (len_C (heap_WordArray_u32_C s (t5_C.arr_C x'))))" and
+                       arr = "(ptr_val (values_C (heap_WordArray_u32_C s (t5_C.arr_C x'))))" and
+                         v = x and \<sigma> = \<sigma> and \<sigma>' = \<sigma> and \<sigma>'' = \<sigma>
+                       in upd_wa_foldnb_bod_0_step; simp)
+         apply (rule u_sem_app)
+           apply (rule u_sem_fun)
+          apply (rule u_sem_var)
+         apply (subst mul_def; clarsimp)
+         apply (rule_tac \<sigma>' = \<sigma> and
+                         fs = "[(UPrim (LU32 x), RPrim (Num U32)),
+                                (UPrim (LU32 (t3_C.acc_C aa)), RPrim (Num U32)),
+                                (UUnit, RUnit)]" in u_sem_take_ub)
+          apply (cut_tac \<xi> = \<xi>0 and 
+                         \<gamma> = "[URecord [(UPrim (LU32 x), RPrim (Num U32)), 
+                                 (UPrim (LU32 (t3_C.acc_C aa)), RPrim (Num U32)), 
+                                 (UUnit, RUnit)]]" and
+                         \<sigma> = \<sigma> and 
+                         i = 0 in u_sem_var; clarsimp)
+         apply clarsimp
+         apply (rule_tac \<sigma>' = \<sigma> and
+                         fs = "[(UPrim (LU32 x), RPrim (Num U32)),
+                                (UPrim (LU32 (t3_C.acc_C aa)), RPrim (Num U32)),
+                                (UUnit, RUnit)]" in u_sem_take_ub)
+          apply (cut_tac \<xi> = \<xi>0 and 
+                         \<gamma> = "[UPrim (LU32 x), 
+                               URecord [(UPrim (LU32 x), RPrim (Num U32)), 
+                                 (UPrim (LU32 (t3_C.acc_C aa)), RPrim (Num U32)), (UUnit, RUnit)],
+                               URecord [(UPrim (LU32 x), RPrim (Num U32)), 
+                                 (UPrim (LU32 (t3_C.acc_C aa)), RPrim (Num U32)), 
+                                 (UUnit, RUnit)]]" and
+                         \<sigma> = \<sigma> and 
+                         i = "Suc 0" in u_sem_var; clarsimp)
+         apply clarsimp
+         apply (rule_tac \<sigma>' = \<sigma> and
+                         fs = "[(UPrim (LU32 x), RPrim (Num U32)),
+                                (UPrim (LU32 (t3_C.acc_C aa)), RPrim (Num U32)),
+                                (UUnit, RUnit)]" in u_sem_take_ub)
+            apply (cut_tac \<xi> = \<xi>0 and 
+                         \<gamma> = "[UPrim (LU32 (t3_C.acc_C aa)),
+                               URecord [(UPrim (LU32 x), RPrim (Num U32)), 
+                                 (UPrim (LU32 (t3_C.acc_C aa)), RPrim (Num U32)), (UUnit, RUnit)],
+                               UPrim (LU32 x),
+                               URecord [(UPrim (LU32 x), RPrim (Num U32)), 
+                                 (UPrim (LU32 (t3_C.acc_C aa)), RPrim (Num U32)), 
+                                 (UUnit, RUnit)],
+                               URecord [(UPrim (LU32 x), RPrim (Num U32)), 
+                                 (UPrim (LU32 (t3_C.acc_C aa)), RPrim (Num U32)), 
+                                 (UUnit, RUnit)]]" and
+                         \<sigma> = \<sigma> and 
+                         i = "Suc 0" in u_sem_var; clarsimp)
+         apply clarsimp
+         apply (cut_tac \<xi> = \<xi>0 and 
+                        \<gamma> = "[UUnit, 
+                              URecord [(UPrim (LU32 x), RPrim (Num U32)),
+                                 (UPrim (LU32 (t3_C.acc_C aa)), RPrim (Num U32)), (UUnit, RUnit)],
+                              UPrim (LU32 (t3_C.acc_C aa)),
+                              URecord [(UPrim (LU32 x), RPrim (Num U32)), 
+                                 (UPrim (LU32 (t3_C.acc_C aa)), RPrim (Num U32)), (UUnit, RUnit)],
+                              UPrim (LU32 x),
+                              URecord [(UPrim (LU32 x), RPrim (Num U32)),
+                                 (UPrim (LU32 (t3_C.acc_C aa)), RPrim (Num U32)), (UUnit, RUnit)],
+                              URecord [(UPrim (LU32 x), RPrim (Num U32)),
+                                 (UPrim (LU32 (t3_C.acc_C aa)), RPrim (Num U32)),
+                                 (UUnit, RUnit)]]" and
+                        \<sigma> = \<sigma> and 
+                       \<sigma>' = \<sigma> and
+                        p = "Times U32" and
+                       as = "[Var 4, Var 2]"  in u_sem_prim)
+          apply (rule u_sem_all_cons)
+           apply (rule u_sem_var)
+          apply (rule u_sem_all_cons)
+           apply (rule u_sem_var)
+          apply (rule u_sem_all_empty)
+         apply (clarsimp simp: eval_prim_u_def val_rel_simps)
+        apply (rule conjI)  
+         apply (metis (no_types, hide_lams) max_word_max word_Suc_le word_le_less_eq word_not_le)
+        apply (rule conjI)
+         apply clarsimp
+         apply (metis (no_types, hide_lams) max_word_max word_Suc_le word_not_le)
+        apply (rule conjI)
+         apply (meson min_less_iff_conj word_not_le)
+        apply (metis (no_types, hide_lams) add.commute diff_less_mono2 max_word_max unat_mono word_Suc_le word_le_less_eq word_less_nat_alt word_not_le)
+       apply (rule conjI)
+        apply (rule_tac r = "UPrim (LU32 (t3_C.acc_C aa))" and 
+                      len = "(SCAST(32 signed \<rightarrow> 32) (len_C (heap_WordArray_u32_C s (t5_C.arr_C x'))))" and
+                      arr = "(ptr_val (values_C (heap_WordArray_u32_C s (t5_C.arr_C x'))))" and
+                        v = x and \<sigma> = \<sigma> and \<sigma>' = \<sigma> and \<sigma>'' = \<sigma>
+                      in upd_wa_foldnb_bod_0_step; simp)
+        apply (rule u_sem_app)
+          apply (rule u_sem_fun)
+         apply (rule u_sem_var)
+        apply (subst sum_def; clarsimp)
+        apply (rule_tac \<sigma>' = \<sigma> and
+                        fs = "[(UPrim (LU32 x), RPrim (Num U32)),
+                               (UPrim (LU32 (t3_C.acc_C aa)), RPrim (Num U32)),
+                               (UUnit, RUnit)]" in u_sem_take_ub)
+         apply (cut_tac \<xi> = \<xi>0 and 
+                        \<gamma> = "[URecord [(UPrim (LU32 x), RPrim (Num U32)), 
+                                (UPrim (LU32 (t3_C.acc_C aa)), RPrim (Num U32)), 
+                                (UUnit, RUnit)]]" and
+                        \<sigma> = \<sigma> and 
+                        i = 0 in u_sem_var; clarsimp)
+        apply clarsimp
+        apply (rule_tac \<sigma>' = \<sigma> and
+                        fs = "[(UPrim (LU32 x), RPrim (Num U32)),
+                               (UPrim (LU32 (t3_C.acc_C aa)), RPrim (Num U32)),
+                               (UUnit, RUnit)]" in u_sem_take_ub)
+         apply (cut_tac \<xi> = \<xi>0 and 
+                        \<gamma> = "[UPrim (LU32 x), 
+                              URecord [(UPrim (LU32 x), RPrim (Num U32)), 
+                                (UPrim (LU32 (t3_C.acc_C aa)), RPrim (Num U32)), (UUnit, RUnit)],
+                              URecord [(UPrim (LU32 x), RPrim (Num U32)), 
+                                (UPrim (LU32 (t3_C.acc_C aa)), RPrim (Num U32)), 
+                                (UUnit, RUnit)]]" and
+                        \<sigma> = \<sigma> and 
+                        i = "Suc 0" in u_sem_var; clarsimp)
+        apply clarsimp
+        apply (rule_tac \<sigma>' = \<sigma> and
+                        fs = "[(UPrim (LU32 x), RPrim (Num U32)),
+                               (UPrim (LU32 (t3_C.acc_C aa)), RPrim (Num U32)),
+                               (UUnit, RUnit)]" in u_sem_take_ub)
+           apply (cut_tac \<xi> = \<xi>0 and 
+                        \<gamma> = "[UPrim (LU32 (t3_C.acc_C aa)),
+                              URecord [(UPrim (LU32 x), RPrim (Num U32)), 
+                                (UPrim (LU32 (t3_C.acc_C aa)), RPrim (Num U32)), (UUnit, RUnit)],
+                              UPrim (LU32 x),
+                              URecord [(UPrim (LU32 x), RPrim (Num U32)), 
+                                (UPrim (LU32 (t3_C.acc_C aa)), RPrim (Num U32)), 
+                                (UUnit, RUnit)],
+                              URecord [(UPrim (LU32 x), RPrim (Num U32)), 
+                                (UPrim (LU32 (t3_C.acc_C aa)), RPrim (Num U32)), 
+                                (UUnit, RUnit)]]" and
+                        \<sigma> = \<sigma> and 
+                        i = "Suc 0" in u_sem_var; clarsimp)
+        apply clarsimp
+        apply (cut_tac \<xi> = \<xi>0 and 
+                       \<gamma> = "[UUnit, 
+                             URecord [(UPrim (LU32 x), RPrim (Num U32)),
+                                (UPrim (LU32 (t3_C.acc_C aa)), RPrim (Num U32)), (UUnit, RUnit)],
+                             UPrim (LU32 (t3_C.acc_C aa)),
+                             URecord [(UPrim (LU32 x), RPrim (Num U32)), 
+                                (UPrim (LU32 (t3_C.acc_C aa)), RPrim (Num U32)), (UUnit, RUnit)],
+                             UPrim (LU32 x),
+                             URecord [(UPrim (LU32 x), RPrim (Num U32)),
+                                (UPrim (LU32 (t3_C.acc_C aa)), RPrim (Num U32)), (UUnit, RUnit)],
+                             URecord [(UPrim (LU32 x), RPrim (Num U32)),
+                                (UPrim (LU32 (t3_C.acc_C aa)), RPrim (Num U32)),
+                                (UUnit, RUnit)]]" and
+                       \<sigma> = \<sigma> and 
+                      \<sigma>' = \<sigma> and
+                       p = "Plus U32" and
+                      as = "[Var 4, Var 2]"  in u_sem_prim)
+         apply (rule u_sem_all_cons)
+          apply (rule u_sem_var)
+         apply (rule u_sem_all_cons)
+          apply (rule u_sem_var)
+         apply (rule u_sem_all_empty)
+        apply (clarsimp simp: eval_prim_u_def val_rel_simps)  
+       apply (rule conjI)  
+        apply (metis (no_types, hide_lams) max_word_max word_Suc_le word_le_less_eq word_not_le)
+       apply (rule conjI)
+        apply clarsimp
+        apply (metis (no_types, hide_lams) max_word_max word_Suc_le word_not_le)
+       apply (rule conjI)
+        apply (meson min_less_iff_conj word_not_le)
+       apply (metis (no_types, hide_lams) add.commute diff_less_mono2 max_word_max unat_mono word_Suc_le word_le_less_eq word_less_nat_alt word_not_le)
+      apply (case_tac a; clarsimp simp: abs_typing_u_def)
+      apply (thin_tac "_ \<in> state_rel")
+      apply (clarsimp simp: state_rel_def heap_rel_def heap_rel_ptr_meta heap_rel_ptr_w32_meta)
+      apply (drule_tac p = "t5_C.arr_C x'" and uv = "UAbstract (WAU32 x11 x12)" in all_heap_rel_ptrD; 
+             clarsimp simp: type_rel_simps is_valid_simp heap_simp abs_repr_u_def val_rel_simps) 
+      apply (thin_tac "cogent_function_val_rel _ _")
+      apply (thin_tac "upd.uval_typing _ _ _ _ _ _")
+      apply clarsimp
+      apply (case_tac "t5_C.to_C x' = b")
+       apply clarsimp
+      apply (case_tac "b < t5_C.to_C x'")
+       apply clarsimp
+       apply (drule_tac arr = "ptr_val (values_C (heap_WordArray_u32_C s (t5_C.arr_C x')))" and 
+                       len = "SCAST(32 signed \<rightarrow> 32) (len_C (heap_WordArray_u32_C s (t5_C.arr_C x')))" 
+                       in upd_wa_foldnb_bod_0_to_geq_lenD)
+         apply simp
+        apply auto[1]
+       apply (rule_tac arr = "ptr_val (values_C (heap_WordArray_u32_C s (t5_C.arr_C x')))" and 
+                       len = "SCAST(32 signed \<rightarrow> 32) (len_C (heap_WordArray_u32_C s (t5_C.arr_C x')))" 
+                       in upd_wa_foldnb_bod_0_to_geq_len; simp)
+      apply clarsimp
+      apply (case_tac "min (t5_C.to_C x') (SCAST(32 signed \<rightarrow> 32) (len_C (heap_WordArray_u32_C s (t5_C.arr_C x')))) \<le> t5_C.frm_C x'")
+       apply clarsimp
+       apply (erule upd_wa_foldnb_bod_0.elims; clarsimp)
+       apply (clarsimp simp: min_def split: if_splits)
+        apply (subst upd_wa_foldnb_bod_0.simps; clarsimp)
+       apply (subst upd_wa_foldnb_bod_0.simps; clarsimp)
+      apply clarsimp
+      apply (rule FalseE)
+      apply (meson min_less_iff_disj not_less word_le_less_eq)
+     apply wp
+    apply wp
+   apply clarsimp
+   apply (subst unknown_def[symmetric])
+   apply (rule validNF_unknown)
+  apply clarsimp
+  apply (subst upd_wa_foldnb_bod_0.simps)
+  apply clarsimp
+  apply (subst upd_wa_foldnb_bod_0.simps)
+  apply clarsimp
+  apply (clarsimp simp: state_rel_def heap_rel_def heap_rel_ptr_meta abs_typing_u_def)
+  apply (case_tac a; clarsimp)
+  apply (drule_tac p = "t5_C.arr_C x'" and uv = "UAbstract (WAU32 x11 x12)" in all_heap_rel_ptrD;
+         clarsimp simp: abs_repr_u_def type_rel_simps is_valid_simp)
+  apply (thin_tac "upd.uval_typing _ _ _ _ _ _")
+  apply (thin_tac "is_valid_WordArray_u32_C _ _")
+  apply (thin_tac "val_rel _ _")
   apply (clarsimp simp: cogent_function_val_rel
                         FUN_ENUM_sum_def
                         FUN_ENUM_dec_def
@@ -185,137 +753,9 @@ gets (\<lambda>s. x)
                         FUN_ENUM_wordarray_get_u32_def
                         FUN_ENUM_wordarray_length_u32_def
                         FUN_ENUM_wordarray_put2_u32_def)
-*)
-  apply (erule upd.u_t_recE)
-  apply (clarsimp simp: \<Xi>_def wordarray_fold_no_break_0_type_def abbreviatedType1_def)
-  apply (erule upd.u_t_r_consE; clarsimp)
-  apply (erule upd.u_t_p_absE; clarsimp simp: abs_typing_u_def)
-  apply (case_tac a; clarsimp)
-  apply (erule upd.u_t_r_consE; clarsimp)
-  apply (erule upd.u_t_primE; subst (asm) lit_type.simps; clarsimp)
-  apply (erule upd.u_t_r_consE; clarsimp)
-  apply (erule upd.u_t_primE; subst (asm) lit_type.simps; clarsimp)
-  apply (erule upd.u_t_r_consE; clarsimp)
-  apply (erule upd.u_t_r_consE; clarsimp)
-  apply (erule upd.u_t_primE; subst (asm) lit_type.simps; clarsimp)
-  apply (erule upd.u_t_r_consE; clarsimp)
-  apply (erule upd.u_t_r_emptyE)
-  apply (erule upd.u_t_unitE)
-  apply (case_tac "sint (t5_C.f_C x') \<noteq> sint FUN_ENUM_mul")
-   apply (case_tac "sint (t5_C.f_C x') \<noteq> sint FUN_ENUM_sum")
-    apply (clarsimp simp: cogent_function_val_rel
-                          FUN_ENUM_sum_def
-                          FUN_ENUM_dec_def
-                          FUN_ENUM_inc_def
-                          FUN_ENUM_mul_def
-                          FUN_ENUM_dec_arr_def
-                          FUN_ENUM_inc_arr_def
-                          FUN_ENUM_mul_arr_def
-                          FUN_ENUM_sum_arr_def
-                          FUN_ENUM_wordarray_get_0_def
-                          FUN_ENUM_wordarray_length_0_def
-                          FUN_ENUM_wordarray_put2_0_def
-                          FUN_ENUM_wordarray_fold_no_break_0_def
-                          FUN_ENUM_wordarray_map_no_break_0_def
-                          FUN_ENUM_wordarray_get_u32_def
-                          FUN_ENUM_wordarray_length_u32_def
-                          FUN_ENUM_wordarray_put2_u32_def)
+  apply (erule disjE; clarsimp)
+   apply (metis (no_types, hide_lams) min.strict_order_iff min_def_raw not_less_iff_gr_or_eq)+
+  done
 
-    apply (rule FalseE)
-    apply (erule disjE)
-     apply (clarsimp simp: dec_def)
-     apply (erule upd.u_t_functionE)
-     apply (erule typing_takeE)+
-     apply (erule typing_letE)+
-     apply (erule typing_structE)
-     apply (erule typing_all_consE)+
-     apply (erule typing_varE)+
-     apply (clarsimp simp: subtyping_simps(4) subtyping.simps[of _ _ "TPrim (Num U32)", simplified])
-    apply (erule disjE)
-     apply (clarsimp simp: inc_def)
-     apply (erule upd.u_t_functionE)
-     apply (erule typing_takeE)+
-     apply (erule typing_letE)+
-     apply (erule typing_structE)
-     apply (erule typing_all_consE)+
-     apply (erule typing_varE)+
-     apply (clarsimp simp: subtyping_simps(4) subtyping.simps[of _ _ "TPrim (Num U32)", simplified])
-    apply (erule disjE)
-     apply (clarsimp simp: dec_arr_def)
-     apply (erule upd.u_t_functionE; clarsimp)
-     apply (erule typing_letE)
-     apply (erule typing_letbE)
-     apply (erule typing_letE)+
-     apply (erule typing_appE)+
-     apply (erule typing_afunE)+
-     apply (clarsimp simp: wordarray_map_no_break_0_type_def abbreviatedType2_def)
-     apply (clarsimp simp: subtyping_simps(4) subtyping.simps[of _ _ "TPrim (Num U32)", simplified])
-    apply (erule disjE)
-     apply (clarsimp simp: inc_arr_def)
-     apply (erule upd.u_t_functionE; clarsimp)
-     apply (erule typing_letE)
-     apply (erule typing_letbE)
-     apply (erule typing_letE)+
-     apply (erule typing_appE)+
-     apply (erule typing_afunE)+
-     apply (clarsimp simp: wordarray_map_no_break_0_type_def abbreviatedType2_def)
-     apply (clarsimp simp: subtyping_simps(4) subtyping.simps[of _ _ "TPrim (Num U32)", simplified])
-    apply (erule disjE)
-     apply (clarsimp simp: mul_arr_def)
-     apply (erule upd.u_t_functionE; clarsimp)
-     apply (clarsimp simp: subtyping_simps(4) subtyping.simps[of _ _ "TPrim (Num U32)", simplified])
-     apply (erule subtyping.cases; clarsimp)
-     apply (subst (asm) subtyping.simps[of _ "TPrim (Num U32)", simplified])+
-     apply (clarsimp simp: subtyping.simps[of _ "TUnit", simplified] kinding_simps(5, 9))
-     apply (erule typing_letE)+
-     apply (erule typing_structE)
-     apply (erule typing_all_consE)+
-     apply (erule typing_all_emptyE)
-     apply (erule typing_varE)+
-     apply (erule typing_litE)+
-     apply (erule typing_unitE)+
-     apply clarsimp
-     apply (erule typing_appE)+
-     apply (erule typing_funE)+
-     apply (clarsimp simp: wordarray_length_u32_def mul_def)
-     apply (erule typing_letE)
-     apply (erule typing_appE)
-     apply (erule typing_afunE)+
-     apply clarsimp
-     apply (erule typing_takeE)+
-     apply (erule typing_primE)
-     apply (erule typing_all_consE)+
-     apply (erule typing_all_emptyE)
-     apply (erule typing_varE)+
-     apply (clarsimp simp: wordarray_length_0_type_def)
-     apply (subst (asm) split_conv_all_nth)
-     apply clarsimp
-     apply (erule split_comp.cases; clarsimp)
-  apply (subst (asm) weakening_conv_all_nth)
-(*
-     apply (case_tac \<Gamma>1; clarsimp)
-     apply (case_tac \<Gamma>2)
-      apply clarsimp
-  find_theorems "split_comp"
-*)
-
-
-(*
-     apply (case_tac \<Gamma>1; clarsimp)
-
-*)
-(*
-     apply (case_tac \<Gamma>2; clarsimp)
-     
-     apply (case_tac a; clarsimp)
-*)
-
-(*
-     apply (clarsimp simp: split_conv_all_nth  weakening_conv_all_nth)
-*)
-
-
-
-  oops
 end (* of context *)
 end
